src/Switched2.v
@@ -7,6 +7,7 @@ Require Import oeuf.Utopia.
 Require Import oeuf.Monads.
 Require Export oeuf.HigherValue.
 Require Import oeuf.AllValues.
+Require Import oeuf.OpaqueOps.
 
 Definition function_name := nat.
 
@@ -19,6 +20,7 @@ Inductive expr :=
 | MkConstr (tag : nat) (args : list expr)
 | Switch (cases : list expr)
 | MkClose (f : function_name) (free : list expr)
+| OpaqueOp (op : opaque_oper_name) (args : list expr)
 .
 
 Definition env := list expr.
@@ -74,6 +76,16 @@ Inductive sstep (E : env) : state -> state -> Prop :=
 | SConstrDone : forall fname vs a s k,
         let es := map Value vs in
         sstep E (Run (MkConstr fname es) a s k) (k (Constr fname vs))
+
+| SOpaqueOpStep : forall op vs e es a s k,
+        Forall is_value vs ->
+        ~ is_value e ->
+        sstep E (Run (OpaqueOp op (vs ++ [e] ++ es)) a s k)
+                (Run e a s (fun v => Run (OpaqueOp op (vs ++ [Value v] ++ es)) a s k))
+| SOpaqueOpDone : forall op vs a s k v,
+        let es := map Value vs in
+        opaque_oper_denote_higher op vs = Some v ->
+        sstep E (Run (OpaqueOp op es) a s k) (k v)
 
 | SCallL : forall e1 e2 a s k,
         ~ is_value e1 ->
@@ -155,6 +167,7 @@ Definition expr_rect_mut
     (HConstr :  forall tag args, Pl args -> P (MkConstr tag args))
     (HSwitch :  forall cases, Pl cases -> P (Switch cases))
     (HClose :   forall f free, Pl free -> P (MkClose f free))
+    (HOpaqueOp : forall o args, Pl args -> P (OpaqueOp o args))
     (Hnil :     Pl [])
     (Hcons :    forall e es, P e -> Pl es -> Pl (e :: es))
     (e : expr) : P e :=
@@ -173,15 +186,16 @@ Definition expr_rect_mut
         | MkConstr tag args => HConstr tag args (go_list args)
         | Switch cases => HSwitch cases (go_list cases)
         | MkClose f free => HClose f free (go_list free)
+        | OpaqueOp o args => HOpaqueOp o args (go_list args)
         end in go e.
 
 Definition expr_rect_mut'
         (P : expr -> Type)
         (Pl : list expr -> Type)
-    HValue HArg HSelf HDeref HCall HConstr HSwitch HClose Hnil Hcons
+    HValue HArg HSelf HDeref HCall HConstr HSwitch HClose HOpaqueOp Hnil Hcons
     : (forall e, P e) * (forall es, Pl es) :=
     let go := expr_rect_mut P Pl
-        HValue HArg HSelf HDeref HCall HConstr HSwitch HClose Hnil Hcons
+        HValue HArg HSelf HDeref HCall HConstr HSwitch HClose HOpaqueOp Hnil Hcons
     in
     let fix go_list es :=
         match es as es_ return Pl es_ with
@@ -200,9 +214,10 @@ Definition expr_ind' (P : expr -> Prop)
     (HConstr :  forall c args, Forall P args -> P (MkConstr c args))
     (HSwitch :  forall cases, Forall P cases -> P (Switch cases))
     (HClose :   forall f free, Forall P free -> P (MkClose f free))
+    (HOpaqueOp : forall o args, Forall P args -> P (OpaqueOp o args))
     (e : expr) : P e :=
     ltac:(refine (@expr_rect_mut P (Forall P)
-        HValue HArg HSelf HDeref HCall HConstr HSwitch HClose _ _ e); eauto).
+        HValue HArg HSelf HDeref HCall HConstr HSwitch HClose HOpaqueOp _ _ e); eauto).
 
 
 
@@ -231,6 +246,7 @@ Definition cases_arent_values : expr -> Prop :=
                 Forall (fun e => ~ is_value e) cases /\
                 go_list cases
         | MkClose _ free => go_list free
+        | OpaqueOp _ args => go_list args
         end in go.
 
 Definition cases_arent_values_list : list expr -> Prop :=
@@ -302,6 +318,17 @@ simpl in *; refold_cases_arent_values.
 
 - eauto.
 
+- rewrite cases_arent_values_list_is_Forall in *.
+  on _, invc_using Forall_app_inv.
+  on (Forall _ (_ :: _)), invc.
+
+  i_ctor. i_ctor. refold_cases_arent_values.
+
+  rewrite cases_arent_values_list_is_Forall.
+  i_lem Forall_app. i_ctor.
+
+- eauto.
+
 - break_and. i_ctor. i_ctor.
 
 - break_and. i_ctor. i_ctor.
@@ -340,6 +367,7 @@ Definition no_values : expr -> Prop :=
         | MkConstr _ args => go_list args
         | Switch cases => go_list cases
         | MkClose _ free => go_list free
+        | OpaqueOp _ args => go_list args
         end in go.
 
 Definition no_values_list : list expr -> Prop :=
