src/Tagged.v
@@ -454,51 +454,33 @@ Defined.
 
 
 Lemma nfree_ok_value_list_Forall : forall nfrees es,
-    nfree_ok_value_list nfrees es ->
+    nfree_ok_value_list nfrees es <->
     Forall (nfree_ok_value nfrees) es.
-induction es; intro HH; simpl in *.
+induction es; split; intro HH; simpl in *.
 - constructor.
-- break_and. constructor; eauto.
-Qed.
-
-Lemma nfree_ok_value_list_Forall' : forall nfrees es,
-    Forall (nfree_ok_value nfrees) es ->
-    nfree_ok_value_list nfrees es.
-induction es; intro HH; simpl in *.
 - constructor.
-- on (Forall _ _), invc. constructor; eauto.
+- break_and. constructor; tauto.
+- on (Forall _ _), invc. constructor; tauto.
 Qed.
 
 Lemma nfree_ok_list_Forall : forall nfrees es,
-    nfree_ok_list nfrees es ->
+    nfree_ok_list nfrees es <->
     Forall (nfree_ok nfrees) es.
-induction es; intro HH; simpl in *.
+induction es; split; intro HH; simpl in *.
 - constructor.
-- break_and. constructor; eauto.
-Qed.
-
-Lemma nfree_ok_list_Forall' : forall nfrees es,
-    Forall (nfree_ok nfrees) es ->
-    nfree_ok_list nfrees es.
-induction es; intro HH; simpl in *.
 - constructor.
-- on (Forall _ _), invc. constructor; eauto.
+- break_and. constructor; tauto.
+- on (Forall _ _), invc. constructor; tauto.
 Qed.
 
 Lemma nfree_ok_list_pair_Forall : forall nfrees es,
-    nfree_ok_list_pair nfrees es ->
+    nfree_ok_list_pair nfrees es <->
     Forall (nfree_ok_pair nfrees) es.
-induction es; intro HH; simpl in *.
+induction es; split; intro HH; simpl in *.
 - constructor.
-- break_and. constructor; eauto.
-Qed.
-
-Lemma nfree_ok_list_pair_Forall' : forall nfrees es,
-    Forall (nfree_ok_pair nfrees) es ->
-    nfree_ok_list_pair nfrees es.
-induction es; intro HH; simpl in *.
 - constructor.
-- on (Forall _ _), invc. constructor; eauto.
+- break_and. constructor; tauto.
+- on (Forall _ _), invc. constructor; tauto.
 Qed.
 
 Lemma nfree_ok_list_map_value : forall nfrees vs,
@@ -584,45 +566,48 @@ invc STEP; invc II.
 
 - (* SCloseStep *)
   simpl in *. refold_nfree_ok nfrees. break_and.
-  on _, eapply_lem nfree_ok_list_Forall.  on _, invc_using Forall_3part_inv.
+  on _, rewrite_fwd nfree_ok_list_Forall.  on _, invc_using Forall_3part_inv.
   i_ctor. i_ctor.
   simpl. refold_nfree_ok nfrees. split.
   + rewrite app_length in *. simpl in *. assumption.
-  + eapply nfree_ok_list_Forall'. i_lem Forall_app.
+  + rewrite nfree_ok_list_Forall. i_lem Forall_app.
 
 - (* SCloseDone *)
   on _, eapply_.
   simpl in *. refold_nfree_ok nfrees. refold_nfree_ok_value nfrees. break_and.
   subst es.
   split.  { rewrite map_length in *. auto. }
-  eapply nfree_ok_value_list_Forall', nfree_ok_list_map_value, nfree_ok_list_Forall. auto.
+  rewrite nfree_ok_value_list_Forall. eapply nfree_ok_list_map_value.
+  rewrite <- nfree_ok_list_Forall. auto.
 
 - (* SConstrStep *)
   simpl in *. refold_nfree_ok nfrees. break_and.
-  on _, eapply_lem nfree_ok_list_Forall.  on _, invc_using Forall_3part_inv.
+  on _, rewrite_fwd nfree_ok_list_Forall.  on _, invc_using Forall_3part_inv.
   i_ctor. i_ctor.
   simpl. refold_nfree_ok nfrees.
-  eapply nfree_ok_list_Forall'. i_lem Forall_app.
+  rewrite nfree_ok_list_Forall. i_lem Forall_app.
 
 - (* SConstrDone *)
   on _, eapply_.
   simpl in *. refold_nfree_ok nfrees. refold_nfree_ok_value nfrees. break_and.
   subst es.
-  eapply nfree_ok_value_list_Forall', nfree_ok_list_map_value, nfree_ok_list_Forall. auto.
+  rewrite nfree_ok_value_list_Forall. eapply nfree_ok_list_map_value.
+  rewrite <- nfree_ok_list_Forall. auto.
 
 - (* SOpaqueOpStep *)
   simpl in *. refold_nfree_ok nfrees. break_and.
-  on _, eapply_lem nfree_ok_list_Forall.  on _, invc_using Forall_3part_inv.
+  on _, rewrite_fwd nfree_ok_list_Forall.  on _, invc_using Forall_3part_inv.
   i_ctor. i_ctor.
   simpl. refold_nfree_ok nfrees.
-  eapply nfree_ok_list_Forall'. i_lem Forall_app.
+  rewrite nfree_ok_list_Forall. i_lem Forall_app.
 
 - (* SOpaqueOpDone *)
   on _, eapply_.
   simpl in *. refold_nfree_ok nfrees. refold_nfree_ok_value nfrees. break_and.
   subst es.
   eapply opaque_oper_denote_higher_nfree_ok_value; eauto.
-  eapply nfree_ok_value_list_Forall', nfree_ok_list_map_value, nfree_ok_list_Forall. auto.
+  rewrite nfree_ok_value_list_Forall. eapply nfree_ok_list_map_value.
+  rewrite <- nfree_ok_list_Forall. auto.
 
 - (* SCallL *)
   simpl in *. break_and.
@@ -636,7 +621,7 @@ invc STEP; invc II.
   simpl in *. refold_nfree_ok_value nfrees. break_and.
   i_ctor.
   + i_lem Forall_nth_error.
-  + i_ctor. i_lem nfree_ok_value_list_Forall.
+  + i_ctor. rewrite <- nfree_ok_value_list_Forall. eauto.
 
 - (* SElimStep *)
   simpl in *. refold_nfree_ok nfrees. break_and.
@@ -644,12 +629,13 @@ invc STEP; invc II.
 
 - (* SEliminate *)
   simpl in *. refold_nfree_ok nfrees. refold_nfree_ok_value nfrees. break_and.
-  on _, eapply_lem nfree_ok_list_pair_Forall.
+  on _, rewrite_fwd nfree_ok_list_pair_Forall.
   fwd eapply Forall_nth_error with (xs := cases); eauto. simpl in *.
   i_ctor.
   eapply unroll_elim_nfree_ok; [ | | | eauto ]; eauto.
-  + i_lem nfree_ok_value_list_Forall.
-  + intros. simpl. refold_nfree_ok nfrees. eauto using nfree_ok_list_pair_Forall'.
+  + rewrite <- nfree_ok_value_list_Forall. eauto.
+  + intros. simpl. refold_nfree_ok nfrees. split; eauto.
+    rewrite nfree_ok_list_pair_Forall. eauto.
 
 Qed.
 
@@ -658,12 +644,12 @@ Lemma public_value_nfree_ok : forall Ameta v,
     nfree_ok_value (map m_nfree Ameta) v.
 induction v using value_ind'; intros0 Hpub; invc Hpub.
 - simpl. refold_nfree_ok_value (map m_nfree Ameta).
-  eapply nfree_ok_value_list_Forall'.
+  rewrite nfree_ok_value_list_Forall.
   list_magic_on (args, tt).
 - simpl. refold_nfree_ok_value (map m_nfree Ameta).
   split.
   + erewrite map_nth_error; [ | eauto ]. congruence.
-  + eapply nfree_ok_value_list_Forall'.
+  + rewrite nfree_ok_value_list_Forall.
     list_magic_on (free, tt).
 - constructor.
 Qed.
